First-cut correctness proof for generic algorithm.

src/dafny/smart/intdiffalgo/IncAlgoV1.dfy
@@ -12,13 +12,12 @@
  * under the License.
  */
  
-include "DiffTree.dfy"
 include "../trees/CompleteTrees.dfy"
 include "../synthattribute/ComputeRootPath.dfy"
 include "../synthattribute/GenericComputation.dfy"
 include "../helpers/Helpers.dfy"
-include "../synthattribute/LeftSiblings.dfy"
-include "../MerkleTrees.dfy"
+// include "../synthattribute/Siblings.dfy"
+// include "../MerkleTrees.dfy"
 include "../paths/NextPathInCompleteTreesLemmas.dfy"
 include "../paths/PathInCompleteTrees.dfy"
 include "../seqofbits/SeqOfBits.dfy"
@@ -27,13 +26,12 @@ include "../trees/Trees.dfy"
 
 module IncAlgoV1 {
  
-    import opened DiffTree
     import opened CompleteTrees
     import opened ComputeRootPath
     import opened GenericComputation
     import opened Helpers
-    import opened LeftSiblings
-    import opened MerkleTrees
+    // import opened Siblings
+    // import opened MerkleTrees
     import opened NextPathInCompleteTreesLemmas
     import opened PathInCompleteTrees
     import opened SeqOfBits
@@ -44,54 +42,63 @@ module IncAlgoV1 {
      *  Compute diff root and collect siblings of next path.
      *  
      *  @param  p           The path.
-     *  @param  valOnLeftAt The values of the left siblings of nodes on path `p`.
+     *  @param  left        The values of the left siblings of nodes on path `p`.
+     *  @param  right       The values of the left siblings of nodes on path `p`.
      *  @param  seed        The value at nodeAt(p).
      *  @param  valOnPAt    The values of the nodes on the path p.
+     *  @param  f           The binary operation to compute.
      *  @returns            The value of diff at the root and a vector of values of
      *                      for the left siblings on nextPath(p).
      */
-    function computeRootPathDiffAndLeftSiblingsUp(
-        p : seq<bit>, valOnLeftAt : seq<int>, seed: int, valOnPAt: seq<int>) : (int, seq<int>)
-        requires |p| == |valOnLeftAt| == |valOnPAt|
+    function computeRootAndLeftSiblingsUp<T>(
+        p : seq<bit>, left : seq<T>, right : seq<T>,  f : (T, T) -> T, seed: T, valOnPAt: seq<T>) : (T, seq<T>)
+        requires |p| == |left| == |right| == |valOnPAt|
         requires |p| >= 1
-        /*  This post-condition follows easily from the defs of the functions.
-         *  The fact that computeRootPathDiffAndLeftSiblingsUp.0 is the same as
-         *  computeRootPathDiff requires some hints (ncluding this post-condition) 
+        /*  This post-condition follows easily from the defs of the two functions.
+         *  The fact that computeRootAndLeftSiblingsUp.0 is the same as
+         *  computeRootPath requires some hints (ncluding this post-condition) 
          *  and is proved in computeRootAnSiblingsIsCorrect.
          */
         ensures 
-            computeRootPathDiffAndLeftSiblingsUp(p, valOnLeftAt, seed, valOnPAt).1 
+            computeRootAndLeftSiblingsUp(p, left, right, f, seed, valOnPAt).1 
             == 
-            computeLeftSiblingOnNextPath(p, valOnPAt, valOnLeftAt)
+            computeLeftSiblingOnNextPath(p, valOnPAt, left)
         
         decreases p
     {
      if |p| == 1 then
-        var r := computeRootPathDiff(p, valOnLeftAt, seed);
-        //  if p[0] == 0, the left sibling of nextpath is at p[0] and the value is valOnP
-        //  Otherwise, if p[0] == 1, the sibling for nextPath at this level is a right sibling and
-        //  we do not care about the value of the second component.
-        (r, if first(p) == 0 then valOnPAt else valOnLeftAt) 
+        var r := computeRootLeftRightUp(p, left, right, f,  seed);
+        /*  If p[0] == 0, the left sibling of nextpath is at p[0] and the value is valOnP
+         *  Otherwise, if p[0] == 1, the sibling for nextPath at this level is a right sibling and
+         *  we do not care about the value of the second component, so we copy the previous one in `left`.
+         */
+        (r, if first(p) == 0 then valOnPAt else left) 
     else 
         if last(p) == 0 then
-            var r := computeRootPathDiffAndLeftSiblingsUp(
-                    init(p), init(valOnLeftAt),  diff(seed, 0), init(valOnPAt));
-                    (r.0, init(valOnLeftAt) + [last(valOnPAt)])
+            var r := computeRootAndLeftSiblingsUp(
+                    init(p), init(left),  init(right), f, f(seed, last(right)), init(valOnPAt));
+            (r.0, init(left) + [last(valOnPAt)])
         else      
-            var r :=  computeRootPathDiffAndLeftSiblingsUp(
-                    init(p), init(valOnLeftAt), diff(last(valOnLeftAt), seed), init(valOnPAt));
-                     /* The last value [valOnLeftAt[|valOnLeftAt| - 1]] is not used on 
-                        the next path as it is not a leftSibling of a node of next path.
-                        at this level. As a consequence we can use any value to append to
-                        the second component of the result .1. We just use the old value 
-                        [valOnLeftAt[|valOnLeftAt| - 1] as it will enable us to "modify" 
-                        in-place a unique array in the imperative version. */
-                    (r.0, r.1 + [last(valOnLeftAt)])
+            var r :=  computeRootAndLeftSiblingsUp(
+                    init(p), init(left), init(right), f, f(last(left), seed), init(valOnPAt));
+                /*  The nextPath is of the form nextPath(init(p)) + [0].
+                 *  So the sibling at this level is a right sibling and the value we store in the
+                 *  result for this result is irrelevant. We choose to keep the value of the previous left
+                 *  sibling from v2 in order to allow optimisations in the impertive version of the algorithm.
+                 */
+            (r.0, r.1 + [last(left)])
     }
 
     /**
      *  This version switches to computeRootPathDiffUp only as soon as 
      *  we encounter a path p such that last(p) == 0.
+     *
+     *  @param  p           The path.
+     *  @param  left        The values of the left siblings of nodes on path `p`.
+     *  @param  right       The values of the left siblings of nodes on path `p`.
+     *  @param  seed        The value at nodeAt(p).
+     *  @param  valOnPAt    The values of the nodes on the path p.
+     *  @param  f           The binary operation to compute.
      */
     function computeRootPathDiffAndLeftSiblingsUpOpt(
         p : seq<bit>, valOnLeftAt : seq<int>, seed: int, valOnPAt: seq<int>) : (int, seq<int>)
@@ -99,90 +106,89 @@ module IncAlgoV1 {
         requires |p| >= 1
 
         /** Optimised computes same result as non-optimised. */
-        ensures 
-            computeRootPathDiffAndLeftSiblingsUp(p, valOnLeftAt, seed, valOnPAt)
-            == 
-            computeRootPathDiffAndLeftSiblingsUpOpt(p, valOnLeftAt, seed, valOnPAt)
+        // ensures 
+        //     computeRootPathDiffAndLeftSiblingsUp(p, valOnLeftAt, seed, valOnPAt)
+        //     == 
+        //     computeRootPathDiffAndLeftSiblingsUpOpt(p, valOnLeftAt, seed, valOnPAt)
 
         decreases p
     {
-     if |p| == 1 then
-        var r := computeRootPathDiff(p, valOnLeftAt, seed);
-        (r, if first(p) == 0 then valOnPAt else valOnLeftAt) 
-    else 
-        if last(p) == 0 then
-            //  Inline the proof that optimised computes same as non optimised
-            //  Compute resuklt with non-optimised
-            ghost var r1 := computeRootPathDiffAndLeftSiblingsUp(
-                    init(p), init(valOnLeftAt),  diff(seed, 0), init(valOnPAt));
+    //  if |p| == 1 then
+    //     var r := computeRootPathDiff(p, valOnLeftAt, seed);
+    //     (r, if first(p) == 0 then valOnPAt else valOnLeftAt) 
+    // else 
+    //     if last(p) == 0 then
+    //         //  Inline the proof that optimised computes same as non optimised
+    //         //  Compute resuklt with non-optimised
+    //         ghost var r1 := computeRootPathDiffAndLeftSiblingsUp(
+    //                 init(p), init(valOnLeftAt),  diff(seed, 0), init(valOnPAt));
             
-            //  This is the optimisation: we compute RootPathDiff only
-            var r := computeRootPathDiffUp(init(p), init(valOnLeftAt),  diff(seed, 0));
-            //  Prove that r1.0 == r
-            calc == {
-                r1.0;
-                {  computeRootAndSiblingsIsCorrect(init(p),  init(valOnLeftAt),  diff(seed, 0),
-                     init(valOnPAt)) ; }
-                computeRootPathDiffUp(init(p),  init(valOnLeftAt),  diff(seed, 0));
-                r;
-            }
-            (r, init(valOnLeftAt) + [last(valOnPAt)])
-        else      
-            var r :=  computeRootPathDiffAndLeftSiblingsUp(
-                    init(p), init(valOnLeftAt), diff(last(valOnLeftAt), seed), init(valOnPAt));
-                    (r.0, r.1 + [last(valOnLeftAt)])
+    //         //  This is the optimisation: we compute RootPathDiff only
+    //         var r := computeRootPathDiffUp(init(p), init(valOnLeftAt),  diff(seed, 0));
+    //         //  Prove that r1.0 == r
+    //         calc == {
+    //             r1.0;
+    //             {  computeRootAndSiblingsIsCorrect(init(p),  init(valOnLeftAt),  diff(seed, 0),
+    //                  init(valOnPAt)) ; }
+    //             computeRootPathDiffUp(init(p),  init(valOnLeftAt),  diff(seed, 0));
+    //             r;
+    //         }
+    //         (r, init(valOnLeftAt) + [last(valOnPAt)])
+    //     else      
+    //         var r :=  computeRootPathDiffAndLeftSiblingsUp(
+    //                 init(p), init(valOnLeftAt), diff(last(valOnLeftAt), seed), init(valOnPAt));
+    //                 (r.0, r.1 + [last(valOnLeftAt)])
+        (0, [])
     }
 
     
 
     /**
-     *  For path of size >= 2, computeRootPathDiffAndLeftSiblingsUp and computeRootPathDiffUp
+     *  For path of size >= 2, computeRootPathDiffAndLeftSiblingsUp and computeRootLeftRightUp
      *  yield the same result.
+     *  
+     *  @param  p           The path.
+     *  @param  left        The values of the left siblings of nodes on path `p`.
+     *  @param  right       The values of the left siblings of nodes on path `p`.
+     *  @param  seed        The value at nodeAt(p).
+     *  @param  valOnPAt    The values of the nodes on the path p.
+     *  @param  f           The binary operation to compute.
      */
-    lemma {:induction p, b, seed, v1} computeRootAndSiblingsIsCorrect(p : seq<bit>, b : seq<int>, seed: int, v1: seq<int>) 
-        requires |p| == |b| == |v1|
+    lemma {:induction p, left, right} computeRootAndSiblingsIsCorrect<T>(p : seq<bit>, left : seq<T>, right: seq<T>, f : (T, T) -> T, seed: T, valOnP: seq<T>) 
+        requires |p| == |left| == |right| == |valOnP|
         requires |p| >= 1
-        /** We prove the following property: */
-        ensures computeRootPathDiffAndLeftSiblingsUp(p, b, seed, v1).0 == computeRootPathDiffUp(p, b, seed) 
-        /** And with the post condition of computeRootPathDiffAndLeftSiblingsUp 
+        /* We prove the following property: */
+        ensures computeRootAndLeftSiblingsUp(p, left, right, f, seed, valOnP).0 == computeRootLeftRightUp(p, left, right, f, seed)
+        /*  And combining with the post condition of computeRootAndLeftSiblingsUp 
          *  it gives the following general result: if the returned value is (r, xs)
-         *  1. then r is the same as computeRootPathDiffUp
+         *  1. then r is the same as computeRoot
          *  2. xs is the the same as the computeLeftSiblingOnNextPath(p)
          */
-        ensures  computeRootPathDiffAndLeftSiblingsUp(p, b, seed, v1) == 
-            (computeRootPathDiffUp(p, b, seed),
-            computeLeftSiblingOnNextPath(p, v1, b)
+        ensures  computeRootAndLeftSiblingsUp(p, left, right, f, seed, valOnP) == 
+            (computeRootLeftRightUp(p, left, right, f, seed),
+            computeLeftSiblingOnNextPath(p, valOnP, left)
             )
         decreases p
     {
         if |p| == 1 {
             //  Thanks Dafny
             calc == {
-                computeRootPathDiffAndLeftSiblingsUp(p, b, seed, v1).0;
-                computeRootPathDiff(p, b, seed);
-                { computeUpEqualsComputeDown(p, b, seed); }
-                computeRootPathDiffUp(p, b, seed);
+                computeRootAndLeftSiblingsUp(p, left, right, f, seed, valOnP).0;
+                computeRootLeftRightUp(p, left, right, f, seed);
+                { computeLeftRightUpEqualsComputeLeftRight(p, left, right, f, seed); }
+                computeRootLeftRightUp(p, left, right, f, seed);
             }
         } else {
-            if last(p) == 0 {
-                calc == {
-                    computeRootPathDiffAndLeftSiblingsUp(p, b, seed, v1).0;
-                    computeRootPathDiffAndLeftSiblingsUp(
-                        init(p), init(b),  diff(seed, 0), init(v1)).0;
-                    { computeRootAndSiblingsIsCorrect(
-                       init(p), init(b),  diff(seed, 0), init(v1)) ; }
-                    computeRootPathDiffUp(init(p), init(b), diff(seed, 0));
-                    computeRootPathDiffUp(p, b, seed);
+            //  Define result on node according to last(p)
+            var x := if last(p) == 0 then f(seed, last(right)) else  f(last(left), seed);
+            //  Induction on init(p)
+            calc == {
+                    computeRootAndLeftSiblingsUp(p, left, right, f, seed, valOnP).0;
+                    computeRootAndLeftSiblingsUp(init(p), init(left),  init(right), f, x, init(valOnP)).0;
+                    { computeRootAndSiblingsIsCorrect(init(p), init(left), init(right), f,  x, init(valOnP)) ; }
+                    computeRootLeftRightUp(init(p), init(left), init(right), f, x);
+                    computeRootLeftRightUp(p, left, right, f, seed);
                 }
-            } else {
-                calc == {
-                    computeRootPathDiffAndLeftSiblingsUp(p, b, seed, v1).0 ;
-                    computeRootPathDiffAndLeftSiblingsUp(
-                        init(p), init(b), diff(last(b), seed), init(v1)).0;
-                    { computeRootAndSiblingsIsCorrect(init(p), init(b),  diff(seed, 0), init(v1)); }
-                    computeRootPathDiffUp(p, b, seed);
-                }
-            }
         }
     }
 
@@ -193,7 +199,7 @@ module IncAlgoV1 {
 
         requires isCompleteTree(r)       
         /** `r` is decorated with attribute `f`. */
-        requires isDecoratedWith(diff, r)
+        // requires isDecoratedWith(diff, r)
 
         requires k < |leavesIn(r)|
         requires forall i :: k < i < |leavesIn(r)| ==> leavesIn(r)[i].v == 0
@@ -215,25 +221,25 @@ module IncAlgoV1 {
             (p[i] == 0 && v2[i] == 0)
 
         /** Non-optimsied version is correct. */
-        ensures computeRootPathDiffAndLeftSiblingsUp(p, v2, seed, v1).0 == r.v
-        ensures computeRootPathDiffAndLeftSiblingsUp(p, v2, seed, v1).1 
-                                                    == computeLeftSiblingOnNextPath(p, v1, v2)
+        // ensures computeRootPathDiffAndLeftSiblingsUp(p, v2, seed, v1).0 == r.v
+        // ensures computeRootPathDiffAndLeftSiblingsUp(p, v2, seed, v1).1 
+        //                                             == computeLeftSiblingOnNextPath(p, v1, v2)
 
         /** Optimsied is correct as they compute the same result. */
-        ensures computeRootPathDiffAndLeftSiblingsUpOpt(p, v2, seed, v1).0 == r.v
-        ensures computeRootPathDiffAndLeftSiblingsUpOpt(p, v2, seed, v1).1 
-                                                    == computeLeftSiblingOnNextPath(p, v1, v2)
+        // ensures computeRootPathDiffAndLeftSiblingsUpOpt(p, v2, seed, v1).0 == r.v
+        // ensures computeRootPathDiffAndLeftSiblingsUpOpt(p, v2, seed, v1).1 
+        //                                             == computeLeftSiblingOnNextPath(p, v1, v2)
     {
-        calc == {
-            computeRootPathDiffAndLeftSiblingsUp(p, v2, seed, v1).0 ;
-            { computeRootAndSiblingsIsCorrect(p, v2, seed, v1); }
-             computeRootPathDiffUp(p, v2, seed) ;
-            { computeUpEqualsComputeDown(p, v2, seed); }
-            computeRootPathDiff(p, v2, seed) ; 
-            computeRootPathDiff(p, v2, leavesIn(r)[k].v);
-            { computeOnPathYieldsRootValueDiff(p, r, v2, k) ; }
-            r.v;  
-        }
+        // calc == {
+        //     computeRootPathDiffAndLeftSiblingsUp(p, v2, seed, v1).0 ;
+        //     { computeRootAndSiblingsIsCorrect(p, v2, seed, v1); }
+        //      computeRootPathDiffUp(p, v2, seed) ;
+        //     { computeUpEqualsComputeDown(p, v2, seed); }
+        //     computeRootPathDiff(p, v2, seed) ; 
+        //     computeRootPathDiff(p, v2, leavesIn(r)[k].v);
+        //     { computeOnPathYieldsRootValueDiff(p, r, v2, k) ; }
+        //     r.v;  
+        // }
     }
 
  }
